More progress on the type soundness theorem.

metatheory/typeSystemScript.sml
@@ -3,6 +3,21 @@ open preamble MiniMLTheory MiniMLTerminationTheory;
 
 val _ = new_theory "typeSystem";
 
+val lookup_zip_map = Q.prove (
+`!x env keys vals res f res'.
+  (LENGTH keys = LENGTH vals) ∧ (env = ZIP (keys,vals)) ∧ (lookup x env = res) ⇒
+  (lookup x (ZIP (keys,MAP f vals)) = OPTION_MAP f res)`,
+recInduct lookup_ind >>
+rw [lookup_def] >>
+cases_on `keys` >>
+cases_on `vals` >>
+fs []);
+
+val option_map_eqns = Q.prove (
+`(!f. option_map f NONE = NONE) ∧
+ (!f x. option_map f (SOME x) = SOME (f x))`,
+rw [option_map_def]);
+
 (* TODO: Move these four definitions to miniML.lem? *)
 (* Check that the dynamic and static constructor environments are consistent *)
 val consistent_con_env_def = Define `
@@ -136,7 +151,7 @@ induct_on `ts'` >>
 rw [] >>
 metis_tac [check_freevars_subst_single]);
 
-val deBruijn_subst_check_freevars = Q.prove (
+val deBruijn_subst_check_freevars = Q.store_thm ("deBruijn_subst_check_freevars",
 `!tvs tvs' t ts.
   check_freevars tvs tvs' t ∧
   EVERY (check_freevars tvs tvs') ts
@@ -405,6 +420,436 @@ every_case_tac >>
 fs [] >>
 metis_tac []);
 
+val deBruijn_subst_tenvE_def = Define `
+(deBruijn_subst_tenvE targs Empty = Empty) ∧
+(deBruijn_subst_tenvE targs (Bind_tvar tvs env) = 
+  Bind_tvar tvs (deBruijn_subst_tenvE targs env)) ∧
+(deBruijn_subst_tenvE targs (Bind_name x tvs t env) =
+  Bind_name x tvs (deBruijn_subst (tvs + num_tvs env) 
+                                  (MAP (deBruijn_inc 0 (tvs + num_tvs env)) targs)
+                                  t)
+       (deBruijn_subst_tenvE targs env))`;
 
+val db_merge_def = Define `
+(db_merge Empty e = e) ∧
+(db_merge (Bind_tvar tvs e1) e2 = Bind_tvar tvs (db_merge e1 e2)) ∧
+(db_merge (Bind_name x tvs t e1) e2 = Bind_name x tvs t (db_merge e1 e2))`;
+
+val num_tvs_db_merge = Q.prove (
+`!e1 e2. num_tvs (db_merge e1 e2) = num_tvs e1 + num_tvs e2`,
+induct_on `e1` >>
+rw [num_tvs_def, db_merge_def] >>
+decide_tac);
+
+val num_tvs_deBruijn_subst_tenvE = Q.prove (
+`!targs tenvE. num_tvs (deBruijn_subst_tenvE targs tenvE) = num_tvs tenvE`,
+induct_on `tenvE` >>
+rw [deBruijn_subst_tenvE_def, num_tvs_def]);
+
+val bind_tvar_rewrites = Q.store_thm ("bind_tvar_rewrites",
+`(!tvs e1 e2. 
+   db_merge (bind_tvar tvs e1) e2 = bind_tvar tvs (db_merge e1 e2)) ∧
+ (!tvs e. num_tvs (bind_tvar tvs e) = tvs + num_tvs e) ∧
+ (!n inc tvs e. lookup_tenv n inc (bind_tvar tvs e) = lookup_tenv n (inc+tvs) e) ∧
+ (!targs tvs e.
+   deBruijn_subst_tenvE targs (bind_tvar tvs e) =
+   bind_tvar tvs (deBruijn_subst_tenvE targs e))`,
+rw [bind_tvar_def, deBruijn_subst_tenvE_def, db_merge_def, num_tvs_def,
+    lookup_tenv_def]);
+
+val lookup_tenv_db_merge = Q.prove (
+`!n inc e1 e2.
+  lookup_tenv n inc (db_merge e1 e2) =
+  case lookup_tenv n inc e1 of
+    | SOME t => SOME t
+    | NONE =>
+        lookup_tenv n (inc + num_tvs e1) e2`,
+induct_on `e1` >>
+rw [lookup_tenv_def, db_merge_def, num_tvs_def] >>
+every_case_tac >>
+srw_tac [ARITH_ss] []);
+
+val tenv_ok_db_merge = Q.prove (
+`!e1 e2. tenv_ok (db_merge e1 e2) ⇒ tenv_ok e2`,
+induct_on `e1` >>
+rw [tenv_ok_def, db_merge_def]);
+
+val check_freevars_deBruijn_inc = Q.prove (
+`!tvs tvs' t. check_freevars tvs tvs' t ⇒ 
+  !n n'. check_freevars (n+tvs) tvs' (deBruijn_inc n' n t)`,
+ho_match_mp_tac check_freevars_ind >>
+rw [check_freevars_def, deBruijn_inc_def] >>
+fs [EVERY_MAP, EVERY_MEM] >>
+rw [check_freevars_def] >>
+decide_tac);
+
+val check_freevars_lem = Q.prove (
+`!l tvs' t.
+  check_freevars l tvs' t ⇒
+  !targs n1 tvs.
+    (l = n1 + (LENGTH targs)) ∧
+    EVERY (check_freevars tvs tvs') targs
+     ⇒
+     check_freevars (n1 + tvs) tvs'
+       (deBruijn_subst n1 (MAP (deBruijn_inc 0 n1) targs) t)`,
+ho_match_mp_tac check_freevars_ind >>
+rw [deBruijn_inc_def, deBruijn_subst_def, check_freevars_def] >|
+[fs [EVERY_MAP, EVERY_MEM] >>
+     metis_tac [],
+ rw [check_freevars_def] >|
+     [fs [EVERY_MEM, MEM_EL] >>
+          `n - n1 < LENGTH targs` by decide_tac >>
+          rw [EL_MAP] >>
+          metis_tac [check_freevars_deBruijn_inc, MEM_EL, 
+                     arithmeticTheory.ADD_COMM, arithmeticTheory.ADD_ASSOC],
+      decide_tac,
+      decide_tac,
+      decide_tac]]);
+
+val type_subst_deBruijn_subst_single = Q.prove (
+`!s t tvs tvs' ts ts' inc.
+  (LENGTH tvs = LENGTH ts) ∧
+  check_freevars 0 tvs t ∧
+  (s = (ZIP (tvs,ts))) ⇒
+  (deBruijn_subst inc ts' (type_subst (ZIP (tvs,ts)) t) =
+   type_subst (ZIP (tvs,MAP (\t. deBruijn_subst inc ts' t) ts)) t)`,
+recInduct type_subst_ind >>
+rw [deBruijn_subst_def, deBruijn_inc_def, type_subst_def, check_freevars_def] >|
+[every_case_tac >>
+     fs [deBruijn_subst_def, deBruijn_inc_def] >|
+     [imp_res_tac lookup_notin >>
+          imp_res_tac MAP_ZIP >>
+          fs [],
+      metis_tac [lookup_zip_map, optionTheory.OPTION_MAP_DEF,
+                 optionTheory.NOT_SOME_NONE],
+      `lookup tv (ZIP (tvs, MAP (λt. deBruijn_subst inc ts' t) ts)) =
+       OPTION_MAP (λt. deBruijn_subst inc ts' t) (SOME x)`
+                     by metis_tac [lookup_zip_map] >>
+          fs []],
+ rw [rich_listTheory.MAP_EQ_f, MAP_MAP_o] >>
+     fs [EVERY_MEM] >>
+     metis_tac []]);
+
+val type_subst_deBruijn_subst_list = Q.prove (
+`!t tvs tvs' ts ts' ts'' inc.
+  (LENGTH tvs = LENGTH ts) ∧
+  EVERY (check_freevars 0 tvs) ts'' ⇒
+  (MAP (deBruijn_subst inc ts') (MAP (type_subst (ZIP (tvs,ts))) ts'') =
+   MAP (type_subst (ZIP (tvs,MAP (\t. deBruijn_subst inc ts' t) ts))) ts'')`,
+induct_on `ts''` >>
+rw [] >>
+metis_tac [type_subst_deBruijn_subst_single]);
+
+val lookup_tenv_subst_none = Q.prove (
+`!n inc e.
+ (lookup_tenv n inc e = NONE) ⇒ 
+ (lookup_tenv n inc (deBruijn_subst_tenvE targs e) = NONE)`,
+induct_on `e` >>
+rw [deBruijn_subst_tenvE_def, lookup_tenv_def]);
+
+val deBruijn_inc_deBruijn_inc = Q.prove (
+`!sk i2 t i1. 
+  deBruijn_inc sk i1 (deBruijn_inc sk i2 t) = deBruijn_inc sk (i1 + i2) t`,
+ho_match_mp_tac deBruijn_inc_ind >>
+rw [deBruijn_inc_def] >>
+rw [] >-
+decide_tac >-
+decide_tac >>
+induct_on `ts` >>
+fs []);
+
+(*
+val deBruijn_subst_inc_lem = Q.prove (
+`(!t ts idx.
+   (deBruijn_subst 0 ts (deBruijn_inc (LENGTH ts) idx t) =
+    deBruijn_subst idx ts (deBruijn_inc 0 idx t))) ∧
+ (!ts' ts idx.
+   (MAP (\t. deBruijn_subst 0 ts (deBruijn_inc (LENGTH ts) idx t)) ts' =
+    MAP (\t. deBruijn_subst idx ts (deBruijn_inc 0 idx t)) ts'))`,
+ho_match_mp_tac t_induction >>
+rw [deBruijn_subst_def, deBruijn_inc_def] >>
+full_simp_tac (srw_ss() ++ ARITH_ss) [MAP_MAP_o, combinTheory.o_DEF]);
+*)
+
+val lookup_tenv_inc_some = Q.prove (
+`!n inc e tvs t inc2.
+   (lookup_tenv n inc e = SOME (tvs, t)) 
+   ⇒
+   ?t'. (t = deBruijn_inc tvs inc t') ∧
+        (lookup_tenv n inc2 e = SOME (tvs, deBruijn_inc tvs inc2 t'))`,
+induct_on `e` >>
+rw [deBruijn_inc_def, lookup_tenv_def] >>
+rw [] >>
+metis_tac [deBruijn_inc_deBruijn_inc]);
+
+val nil_deBruijn_inc = Q.store_thm ("nil_deBruijn_inc",
+`∀skip tvs t. 
+  (check_freevars skip [] t ∨ check_freevars skip [] (deBruijn_inc skip tvs t))
+  ⇒ 
+  (deBruijn_inc skip tvs t = t)`,
+ho_match_mp_tac deBruijn_inc_ind >>
+rw [deBruijn_inc_def, check_freevars_def] >-
+decide_tac >-
+(induct_on `ts` >>
+     rw [] >>
+     metis_tac []) >-
+(induct_on `ts` >>
+     rw [] >>
+     metis_tac []) >>
+metis_tac []);
+
+val nil_deBruijn_subst = Q.store_thm ("nil_deBruijn_subst",
+`∀skip tvs t. check_freevars skip [] t ⇒ (deBruijn_subst skip tvs t = t)`,
+ho_match_mp_tac deBruijn_subst_ind >>
+rw [deBruijn_subst_def, check_freevars_def] >>
+induct_on `ts'` >>
+rw []);
+
+val type_e_subst_lem1 = Q.prove (
+`!e n inc t.
+  (num_tvs e = 0) ∧
+  tenv_ok e ∧
+  (lookup_tenv n inc e = SOME (tvs, deBruijn_inc tvs inc t))
+  ⇒
+  check_freevars tvs [] t`,
+induct_on `e` >>
+rw [lookup_tenv_def, num_tvs_def, tenv_ok_def] >|
+[metis_tac [arithmeticTheory.ADD, arithmeticTheory.ADD_COMM],
+ `check_freevars n [] t0` 
+          by metis_tac [arithmeticTheory.ADD, arithmeticTheory.ADD_COMM] >>
+     fs [nil_deBruijn_inc] >>
+     rw [] >>
+     metis_tac [nil_deBruijn_inc],
+ metis_tac [arithmeticTheory.ADD, arithmeticTheory.ADD_COMM]]);
+
+val type_e_subst_lem2 = Q.prove (
+`(!t sk targs targs' tvs'.
+  check_freevars (LENGTH targs) [] t ⇒
+  (deBruijn_subst sk (MAP (deBruijn_inc 0 sk) targs') (deBruijn_subst 0 targs t) =
+   deBruijn_subst 0 (MAP (deBruijn_subst sk (MAP (deBruijn_inc 0 sk) targs')) targs) t)) ∧
+ (!ts sk targs targs' tvs'.
+  EVERY (check_freevars (LENGTH targs) []) ts ⇒
+  (MAP (deBruijn_subst sk (MAP (deBruijn_inc 0 sk) targs')) (MAP (deBruijn_subst 0 targs) ts) =
+  (MAP (deBruijn_subst 0 (MAP (deBruijn_subst sk (MAP (deBruijn_inc 0 sk) targs')) targs)) ts)))`,
+ho_match_mp_tac t_induction >>
+rw [deBruijn_subst_def, deBruijn_inc_def] >>
+fs [EL_MAP, MAP_MAP_o, combinTheory.o_DEF] >>
+rw [] >>
+full_simp_tac (srw_ss()++ARITH_ss) [deBruijn_subst_def, check_freevars_def] >>
+metis_tac []);
+
+val type_e_subst_lem3 = Q.store_thm ("type_e_subst_lem3",
+`∀tvs tvs2 t.
+  check_freevars tvs tvs2 t ⇒
+  ∀tvs' targs n.
+  (tvs = n + LENGTH targs) ∧
+  EVERY (check_freevars tvs' tvs2) targs
+  ⇒
+  check_freevars (n + tvs') tvs2
+     (deBruijn_subst n (MAP (deBruijn_inc 0 n) targs) t)`,
+ho_match_mp_tac check_freevars_ind >>
+rw [check_freevars_def, deBruijn_inc_def, deBruijn_subst_def, EVERY_MAP] >>
+fs [EVERY_MEM] >>
+rw [] >>
+full_simp_tac (srw_ss()++ARITH_ss) [check_freevars_def, EL_MAP, MEM_EL] >>
+`n - n' < LENGTH targs` by decide_tac >>
+metis_tac [check_freevars_deBruijn_inc]);
+
+val type_e_subst_lem4 = Q.prove (
+`!sk i2 t i1. 
+  deBruijn_inc sk i1 (deBruijn_inc 0 (sk + i2) t) = deBruijn_inc 0 (i1 + (sk + i2)) t`,
+ho_match_mp_tac deBruijn_inc_ind >>
+rw [deBruijn_inc_def] >>
+rw [] >-
+decide_tac >-
+decide_tac >>
+induct_on `ts` >>
+rw []);
+
+val type_e_subst_lem5 = Q.prove (
+`(!t n inc n' targs.
+   deBruijn_inc n inc 
+         (deBruijn_subst (n + n') (MAP (deBruijn_inc 0 (n + n')) targs) t) =
+   deBruijn_subst (n + inc + n') (MAP (deBruijn_inc 0 (n + inc + n')) targs) 
+         (deBruijn_inc n inc t)) ∧
+ (!ts n inc n' targs.
+   MAP (deBruijn_inc n inc)
+         (MAP (deBruijn_subst (n + n') (MAP (deBruijn_inc 0 (n + n')) targs)) ts) =
+   MAP (deBruijn_subst (n + inc + n') (MAP (deBruijn_inc 0 (n + inc + n')) targs))
+         (MAP (deBruijn_inc n inc) ts))`,
+ho_match_mp_tac t_induction >>
+rw [deBruijn_subst_def, deBruijn_inc_def] >>
+rw [] >>
+full_simp_tac (srw_ss()++ARITH_ss) [EL_MAP] >>
+metis_tac [type_e_subst_lem4]);
+
+val type_e_subst_lem6 = Q.prove (
+`!e n inc t tvs.
+  tenv_ok e ∧
+  (lookup_tenv n inc e = SOME (tvs, t))
+  ⇒
+  check_freevars (tvs+inc+num_tvs e) [] t`,
+induct_on `e` >>
+rw [lookup_tenv_def, num_tvs_def, tenv_ok_def] >|
+[metis_tac [arithmeticTheory.ADD_ASSOC],
+ imp_res_tac check_freevars_deBruijn_inc >>
+     metis_tac [arithmeticTheory.ADD_ASSOC, arithmeticTheory.ADD_COMM],
+ metis_tac []]);
+
+val lookup_tenv_deBruijn_subst_tenvE = Q.prove (
+`∀n e targs tvs t inc.
+  (lookup_tenv n inc e = SOME (tvs,t)) 
+  ⇒
+  (lookup_tenv n inc (deBruijn_subst_tenvE targs e) = 
+     SOME (tvs, deBruijn_subst (tvs+inc+num_tvs e) (MAP (deBruijn_inc 0 (tvs+inc+num_tvs e)) targs) t))`,
+induct_on `e` >>
+rw [lookup_tenv_def,deBruijn_subst_tenvE_def, deBruijn_inc_def, num_tvs_def] >>
+metis_tac [arithmeticTheory.ADD_ASSOC, type_e_subst_lem5]);
+
+(*
+val type_e_subst_lem7 = Q.prove (
+`(!t sk targs targs' tvs' tvs''.
+  EVERY (check_freevars (tvs'') []) targs' ∧
+  EVERY (check_freevars (sk + LENGTH targs') []) targs ∧
+  check_freevars (LENGTH targs + sk + tvs'') [] t ⇒
+  (deBruijn_subst sk (MAP (deBruijn_inc 0 sk) targs') (deBruijn_subst 0 targs t) =
+   deBruijn_subst 0 (MAP (deBruijn_subst sk (MAP (deBruijn_inc 0 sk) targs')) targs) 
+     (deBruijn_subst (LENGTH targs + sk) (MAP (deBruijn_inc 0 (LENGTH targs + sk)) targs') t))) ∧
+ (!ts sk targs targs' tvs' tvs''.
+  EVERY (check_freevars (tvs'') []) targs' ∧
+  EVERY (check_freevars (sk + LENGTH targs') []) targs ∧
+  EVERY (check_freevars (LENGTH targs + sk + tvs'') []) ts ⇒
+  (MAP (deBruijn_subst sk (MAP (deBruijn_inc 0 sk) targs')) (MAP (deBruijn_subst 0 targs) ts) =
+  (MAP (deBruijn_subst 0 (MAP (deBruijn_subst sk (MAP (deBruijn_inc 0 sk) targs')) targs))
+       (MAP (deBruijn_subst (LENGTH targs + sk) (MAP (deBruijn_inc 0 (LENGTH targs + sk)) targs')) ts))))`,
+
+ho_match_mp_tac t_induction >>
+rw [deBruijn_subst_def, deBruijn_inc_def] >>
+fs [EL_MAP, MAP_MAP_o, combinTheory.o_DEF] >>
+rw [] >>
+full_simp_tac (srw_ss()++ARITH_ss) [EL_MAP, deBruijn_subst_def, check_freevars_def] >>
+
+metis_tac []);
+
+
+(*
+val deBruijn_subst_order = Q.prove (
+`!sk ts' t.
+  deBruijn_subst 0 (MAP (deBruijn_subst sk (MAP (deBruijn_inc 0 sk) ts')) ts) (deBruijn_subst (LENGTH ts + sk) ts' t)
+  =
+  deBruijn_subst sk (MAP (deBruijn_inc 0 sk) ts') (deBruijn_subst 0 ts t)`,
+
+ho_match_mp_tac deBruijn_subst_ind >>
+rw [deBruijn_subst_def] >>
+rw [] >>
+full_simp_tac (srw_ss() ++ ARITH_ss) [EL_MAP]
+
+decide_tac
+*)
+
+(*
+∃tenv'.
+  type_env tenvC senv env tenv' ∧
+  type_e tenvC
+    (bind_tenv x 0 (deBruijn_subst 0 targs t1) (bind_tvar tvs tenv'))
+    (deBruijn_subst_e 0 targs e) (deBruijn_subst 0 targs t2)
+------------------------------------
+  0.  tenvC_ok tenvC
+  1.  EVERY (check_freevars tvs []) targs
+  2.  check_freevars (LENGTH targs) [] t2
+  3.  type_env tenvC senv env tenv
+  4.  check_freevars (LENGTH targs) [] t1
+  5.  type_e tenvC (bind_tenv x 0 t1 (bind_tvar (LENGTH targs) tenv)) e
+        t2
+        *)
+
+val type_e_subst = Q.prove ("type_e_subst",
+`(!tenvC tenvE e t. type_e tenvC tenvE e t ⇒
+    !tenvE1 targs tvs targs'.
+      (num_tvs tenvE2 = 0) ∧
+      tenvC_ok tenvC ∧
+      tenv_ok tenvE ∧
+      (EVERY (check_freevars tvs []) targs) ∧
+      (tenvE = db_merge tenvE1 (bind_tvar (LENGTH targs) tenvE2)) ∧
+      (targs' = MAP (deBruijn_inc 0 (num_tvs tenvE1)) targs)
+      ⇒
+      type_e tenvC (db_merge (deBruijn_subst_tenvE targs tenvE1) (bind_tvar tvs tenvE2)) 
+                   (deBruijn_subst_e (num_tvs tenvE1) targs' e)
+                   (deBruijn_subst (num_tvs tenvE1) targs' t)) ∧
+ (!tenvC tenvE es ts. type_es tenvC tenvE es ts ⇒
+    !tenvE1 targs tvs targs'.
+      (num_tvs tenvE2 = 0) ∧
+      tenvC_ok tenvC ∧
+      tenv_ok tenvE ∧
+      (EVERY (check_freevars tvs []) targs) ∧
+      (tenvE = db_merge tenvE1 (bind_tvar (LENGTH targs) tenvE2)) ∧
+      (targs' = MAP (deBruijn_inc 0 (num_tvs tenvE1)) targs)
+      ⇒
+    type_es tenvC (db_merge (deBruijn_subst_tenvE targs tenvE1) (bind_tvar tvs tenvE2))
+                  (MAP (deBruijn_subst_e (num_tvs tenvE1) targs') es) 
+                  (MAP (deBruijn_subst (num_tvs tenvE1) targs') ts)) ∧
+ (!tenvC tenvE funs env. type_funs tenvC tenvE funs env ⇒
+    type_funs tenvC tenvE funs env)`,
+
+ho_match_mp_tac type_e_strongind >>
+rw [] >>
+ONCE_REWRITE_TAC [type_e_cases] >>
+rw [deBruijn_subst_e_def, deBruijn_subst_def, deBruijn_subst_tenvE_def, 
+    bind_tvar_rewrites, bind_tenv_def, num_tvs_def, option_map_eqns,
+    num_tvs_db_merge, num_tvs_deBruijn_subst_tenvE] >>
+fs [deBruijn_subst_e_def, deBruijn_subst_def, deBruijn_subst_tenvE_def, 
+    bind_tvar_rewrites, bind_tenv_def, num_tvs_def, option_map_eqns,
+    num_tvs_db_merge, num_tvs_deBruijn_subst_tenvE, tenv_ok_def] >>
+`tenv_ok tenvE2` by metis_tac [tenv_ok_db_merge, bind_tvar_def, tenv_ok_def] >|
+[metis_tac [check_freevars_lem],
+ qpat_assum `!tenvE1' targs' tvs'. P tenvE1' targs' tvs' ⇒
+        type_e tenvC
+          (db_merge (deBruijn_subst_tenvE targs' tenvE1')
+             (bind_tvar tvs' tenvE2))
+          (deBruijn_subst_e (num_tvs tenvE1')
+             (MAP (deBruijn_inc 0 (num_tvs tenvE1')) targs') e')
+          (deBruijn_subst (num_tvs tenvE1')
+             (MAP (deBruijn_inc 0 (num_tvs tenvE1')) targs') t)`
+        (MP_TAC o Q.SPECL [`Bind_name var 0 Tint tenvE1`,
+                           `targs`,
+                           `tvs`]) >>
+     rw [db_merge_def] >>
+     fs [EVERY_MAP, EVERY_MEM, deBruijn_subst_tenvE_def, num_tvs_def,
+         check_freevars_def, db_merge_def, deBruijn_subst_def],
+ fs [EVERY_MAP, EVERY_MEM] >>
+     rw [] >>
+     metis_tac [check_freevars_lem, EVERY_MEM],
+ metis_tac [type_subst_deBruijn_subst_list, tenvC_ok_lookup],
+ imp_res_tac type_e_subst_lem6 >>
+     fs [lookup_tenv_db_merge] >>
+     cases_on `lookup_tenv n 0 tenvE1` >>
+     fs [lookup_tenv_def, bind_tvar_rewrites, num_tvs_deBruijn_subst_tenvE] >>
+     rw [] >|
+     [imp_res_tac lookup_tenv_subst_none >>
+          rw [] >>
+          imp_res_tac lookup_tenv_inc_some >>
+          rw [] >>
+          pop_assum (ASSUME_TAC o Q.SPEC `num_tvs tenvE1 + tvs'`) >>
+          fs [] >>
+          rw [] >>
+          imp_res_tac type_e_subst_lem1 >>
+          fs [nil_deBruijn_inc] >-
+          metis_tac [type_e_subst_lem2] >>
+          fs [EVERY_MAP, EVERY_MEM] >>
+          rw [] >>
+          metis_tac [type_e_subst_lem3, EVERY_MEM],
+      imp_res_tac lookup_tenv_deBruijn_subst_tenvE >>
+          pop_assum (ASSUME_TAC o Q.SPEC `targs'`) >>
+          fs [] >>
+          rw [] >>
+          fs [nil_deBruijn_subst, num_tvs_db_merge, bind_tvar_rewrites] >>
+
+          fs [EVERY_MAP, EVERY_MEM] >>
+          rw [] >>
+          metis_tac [type_e_subst_lem3, EVERY_MEM],
+
+
+
+          *)
 val _ = export_theory ();
 
